template-coq/theories/AstUtils.v
@@ -4,6 +4,8 @@ From Template Require Import Ast utils.
 Import List.ListNotations.
 Require Import FunctionalExtensionality.
 
+Ltac inv H := inversion_clear H.
+
 Definition map_decl f (d : context_decl) :=
   {| decl_name := d.(decl_name);
      decl_body := option_map f d.(decl_body);
@@ -125,10 +127,10 @@ Inductive All (A : Type) (P : A -> Type) : list A -> Type :=
                   P x -> All A P l -> All A P (x :: l).
 Arguments All {A} P l.
 
-Inductive All2 {A B : Type} (R : A -> B -> Type) : list A -> list B -> Type :=
-  All2_nil : All2 R [] []
-| All2_cons : forall (x : A) (y : B) (l : list A) (l' : list B),
-    R x y -> All2 R l l' -> All2 R (x :: l) (y :: l').
+Inductive Forall2 {A B : Type} (R : A -> B -> Type) : list A -> list B -> Type :=
+  Forall2_nil : Forall2 R [] []
+| Forall2_cons : forall (x : A) (y : B) (l : list A) (l' : list B),
+    R x y -> Forall2 R l l' -> Forall2 R (x :: l) (y :: l').
 
 Inductive OnOne2 {A : Type} (P : A -> A -> Type) : list A -> list A -> Type :=
 | OnOne2_hd hd hd' tl : P hd hd' -> OnOne2 P (hd :: tl) (hd' :: tl)
@@ -248,6 +250,25 @@ Proof.
   eapply map_def_spec; eauto.
 Qed.
 
+Lemma Forall_forall_mix {A B : Type} {P : A -> Prop} {p : A -> bool} {l : list A} :
+  Forall P l -> forallb p l = true -> Forall (fun x => P x /\ p x = true) l.
+Proof.
+  induction 1. constructor. simpl. rewrite andb_true_iff. intuition.
+Qed.
+
+Lemma Forall_mix {A} (P Q : A -> Prop) : forall l, Forall P l -> Forall Q l -> Forall (fun x => P x /\ Q x) l.
+Proof.
+  intros l Hl Hq. induction Hl; inv Hq; constructor; auto.
+Qed.
+
+Ltac merge_Forall := unfold tFixProp, tCaseBrsProp in *;
+  repeat match goal with
+  | H : Forall _ ?x, H' : Forall _ ?x |- _ =>
+    apply (Forall_mix _ _ _ H) in H'; clear H
+  | H : Forall _ ?x, H' : forallb _ ?x = _ |- _ =>
+    eapply (Forall_forall_mix H) in H'; clear H
+  end.
+
 Lemma forall_forallb_map_spec {A B : Type} {P : A -> Prop} {p : A -> bool}
       {l : list A} {f g : A -> B} :
     Forall P l -> forallb p l = true ->
@@ -306,8 +327,6 @@ Ltac apply_spec :=
   match goal with
   | H : Forall _ _, H' : forallb _ _ = _ |- map _ _ = map _ _ =>
     eapply (forall_forallb_map_spec H H')
-  | H : Forall _ _ |- map _ _ = map _ _ =>
-    eapply (forall_map_spec H)
   | H : tCaseBrsProp _ _, H' : forallb _ _ = _ |- map _ _ = map _ _ =>
     eapply (case_brs_forallb_map_spec H H')
   | H : tCaseBrsProp _ _ |- map _ _ = map _ _ =>
@@ -316,6 +335,8 @@ Ltac apply_spec :=
     eapply (tfix_forallb_map_spec H H')
   | H : tFixProp _ _ |- map _ _ = map _ _ =>
     eapply (tfix_map_spec H)
+  | H : Forall _ _ |- map _ _ = map _ _ =>
+    eapply (forall_map_spec H)
   end.
 
 Lemma Forall_map {A B} (P : B -> Prop) (f : A -> B) l : Forall (Program.Basics.compose P f) l -> Forall P (map f l).
@@ -347,14 +368,14 @@ Qed.
 
 Lemma Forall2_Forall_left {A B} (P : A -> B -> Type) (Q : A -> Prop) (l : list A) (l' : list B) :
   (forall x y, P x y -> Q x) ->
-  All2 P l l' -> List.Forall Q l.
+  Forall2 P l l' -> List.Forall Q l.
 Proof.
   intros H. induction 1; constructor; eauto.
 Qed.
 
 Lemma Forall2_Forall_right {A B} (P : A -> B -> Type) (Q : B -> Prop) (l : list A) (l' : list B) :
   (forall x y, P x y -> Q y) ->
-  All2 P l l' -> List.Forall Q l'.
+  Forall2 P l l' -> List.Forall Q l'.
 Proof.
   intros H. induction 1; constructor; eauto.
 Qed.
@@ -370,3 +391,90 @@ Lemma Forall2_non_nil {A B} (P : A -> B -> Prop) (l : list A) (l' : list B) :
 Proof.
   induction 1; congruence.
 Qed.
+
+Lemma map_ext {A B : Type} (f g : A -> B) (l : list A) :
+  (forall x, f x = g x) ->
+  map f l = map g l.
+Proof.
+  intros.
+  induction l; trivial.
+  intros. simpl. rewrite H. congruence.
+Defined.
+
+Require Import ssreflect.
+
+Lemma map_skipn {A B} (f : A -> B) (l : list A) (n : nat) : map f (skipn n l) = skipn n (map f l).
+Proof.
+  elim: n l => l // IHn.
+  by case => //.
+Qed.
+
+Lemma nth_error_map {A B} (f : A -> B) n l : nth_error (map f l) n = option_map f (nth_error l n).
+Proof.
+  elim: n l; case => // IHn l /=.
+  - by case: l => //.
+  - by case => //.
+Qed.
+
+Lemma forallb2_Forall {A : Type} {p : A -> A -> bool}
+      {l l' : list A} :
+    forallb2 p l l' = true -> Forall2 (fun x y => p x y = true) l l'.
+Proof.
+  induction l in l' |- *; destruct l'; simpl; intros; try congruence.
+  - constructor.
+  - constructor. revert H; rewrite andb_true_iff; intros [px pl]. auto.
+    apply IHl. revert H; rewrite andb_true_iff; intros [px pl]. auto.
+Qed.
+
+Lemma Forall2_List_Forall_mix {A : Type} {P : A -> Prop} {Q : A -> A -> Prop}
+      {l l' : list A} :
+    List.Forall P l -> Forall2 Q l l' -> Forall2 (fun x y => P x /\ Q x y) l l'.
+Proof.
+  induction 2; simpl; intros; constructor.
+  inv H; intuition auto.
+  apply IHX. inv H; intuition auto.
+Qed.
+
+Lemma Forall2_List_Forall_mix_right {A : Type} {P : A -> Prop} {Q : A -> A -> Prop}
+      {l l' : list A} :
+    List.Forall P l' -> Forall2 Q l l' -> Forall2 (fun x y => P y /\ Q x y) l l'.
+Proof.
+  induction 2; simpl; intros; constructor.
+  inv H; intuition auto.
+  apply IHX. inv H; intuition auto.
+Qed.
+
+Lemma Forall2_Forall_mix {A : Set} {P : A -> Type} {Q : A -> A -> Type}
+      {l l' : list A} :
+  All P l -> Forall2 Q l l' -> Forall2 (fun x y => (P x * Q x y)%type) l l'.
+Proof.
+  induction 2; simpl; intros; constructor.
+  inv X; intuition auto.
+  apply IHX0. inv X; intuition auto.
+Qed.
+
+Lemma map_nil {A B} (f : A -> B) (l : list A) : l <> [] -> map f l <> [].
+Proof. induction l; simpl; congruence. Qed.
+
+Lemma OnOne2_mix_Forall_left {A} {P : A -> A -> Prop} {Q : A -> Prop} {l l'} :
+  List.Forall Q l -> OnOne2 P l l' -> OnOne2 (fun x y => P x y /\ Q x) l l'.
+Proof.
+  intros H; induction 1; constructor; try inv H; intuition.
+  apply IHX. now inv H.
+Qed.
+
+Lemma Forall_skipn {A} (P : A -> Prop) l n : List.Forall P l -> List.Forall P (skipn n l).
+Proof. intros HPL; induction HPL in n |- * ; simpl; destruct n; try econstructor; eauto. Qed.
+
+Lemma nth_error_forall {A} (P : A -> Prop) (l : list A) n x :
+  nth_error l n = Some x -> List.Forall P l -> P x.
+Proof.
+  intros Hnth HPl. induction HPl in n, Hnth |- *. destruct n; discriminate.
+  revert Hnth. destruct n. now intros [= ->].
+  intros H'; eauto.
+Qed.
+
+Lemma All_Forall {A} (P : A -> Type) (Q : A -> Prop) l :
+  (forall x, P x -> Q x) ->
+  All P l -> Forall Q l.
+Proof. induction 2; constructor; auto. Qed.
